# Lambda Calculus

## Introduction
- Works with applications of functions to arguments
- Example
	- Consider the following polynomial: `x^2−2⋅x+5`
	- In lambda calculus, one would represent it as follows: `λx[x^2−2⋅x+5]`
	- The λ operator allows us to abstract over x (it binds the variable to the expression)
- Central principle of lambda calculus is 𝛽-reduction (or 𝛽-conversion). 
	- `(λx[M])N⊳M[x:=N]`
	- We can reduce an application of an abstract term by replacing all instaces of x by N inside M.
	- This reduction is also one of the principles of functional programming. In essence, the abstraction over a given variable can be achieved through functions. As an example consider the following piece of code: `val a = {println(42); 42}`. Replacing a with the value 42 would not yield the same result, as it has the side-effect of printing the number 42 to stdout. Therefore, this is not a pure expression, as it has side-effects and cannot be replaced by its return value.
- Set theory vs. Lambda calculus
	- In set theory, a function is an argument-value pair, meaning: `(x,y)∈𝑓 and (x,z)∈f implies y=z`
		- The function f assigns the value y to the argument x
		- Two functions are identical iff they assign the same values to the same arguments
		- In essence: Functions-as-sets are extensional objects
	- Lambda calculus follows the principle of functions-as-rules
		- A function is given by a rule for how to determine its values from its arguments
		- For instance, the term `λx[M]` can be seen a function that, given 𝑥, produces M.
		- Given rules M and N, we cannot know whether `λx[M]` is equal to `λx[N]`. In other words, functions-as-rules are non-extensional objects (also known as intensional).
	- (In the present possible-worlds terminology, function concepts are classified as extensional or intensional based of their behaviour at possible-worlds. See more info about possible-worlds semantics the [source]( https://plato.stanford.edu/entries/lambda-calculus/))
- *hyperintensional*: A function concept that allows for intensionally equivalent functions to be distinct
	- The point is that in possible-worlds terminology, the function concept at work in the λ-calculus may be regarded not as intentional but *hyperintensional*.
	- As an example, consider the following example:
		- We have the following functions:
			- `ADD-ONE:=λx[x+1]` 
			- `ADD-TWO-SUBTRACT-ONE:=λx[[x+2]−1]`
		- The functions are extensionally equivalent: they assign the same value to the same input at the actual world
		- They are also intentionally equivalent, if we consider that the mathematical facts are the same in every possible world.

## Syntax

<u>Definition</u>
For the alphabet of the language of the λ-calculus we take the left and right parentheses, left and right square brackets, the symbol λ, and an infinite set of variables. The class of λ-terms is defined inductively as follows:
1. Every variable is a λ-term.
2. If M and N are λ-terms, then so is (MN).
3. If M is a λ-term and x is a variable, then `(λx[M])` is a λ-term.
By *term* we always mean λ-term. Terms formed according to rule (2) are called **_application terms_**. Terms formed according to rule (3) are called **_abstraction terms_**.


<u>Definition</u>
The syntactic functions FV and BV (for ‘free variable’ and ‘bound variable’, respectively) are defined on the set of λ𝜆-terms by structural induction thus:

For every variable x𝑥, term M, and term N:

|     | Free                     | Bound                    |
| --- | ------------------------ | ------------------------ |
| 1   | `FV(x)= {x}`             | `BV(x)= ∅`               |
| 2   | `FV(MN)= FV(M) ∪ FV(N)`  | `BV(MN)= BV(M) ∪ BV(N)`  |
| 3   | `FV(λx[M])= FV(M) − {x}` | `BV(λx[M])= BV(M) ∪ {x}` |

If `FV(M)=∅` then M is called a **_combinator_**.


<u>Definition (substitution)</u> 
We write `M[x:=N]` to denote the substitution of N for the free occurrences of x in M. A precise definition by recursion on the set of λ-terms is as follows: for all terms A, B, and M, and for all variables x and y, we define:
1. `x[x:=M] ≡ M` - Replacing the variable with something else will return the newly replaced value
2. `y[x:=M] ≡ y` (y distinct from x) - Nothing happens to y when we replace x (when both variables are different)
3. `(AB)[x:=M] ≡ A[x:=M]B[x:=M]` - Substitution is applied to all terms equally
4. `(λx[A])[x:=M] ≡ λx[A]` - If the bound variable is identical to the variable we are trying to substitute, then we do not perform any substitution. The variable x does not occur freely, so there is nothing to do.
5. `(λy[A])[x:=M] ≡ λy[A[x:=M]]` (y distinct from x) - This is an extension of the previous case, but where x occurs freely and y is a bound variable (x != y). Therefore, we replace all occurrences of x with M in the term A.

<u>Definition (change of bound variables, α-convertibility). </u>
The term N is obtained from the term M by a **_change of bound variables_** if, roughly, any abstraction term `λx[A]` inside M has been replaced by `λy[A[x:=y]]`.

Let us say that terms M and N are α-convertible if there is a sequence of changes of bound variables starting from M and ending at N.

<u>Axiom - β-conversion</u>
`(λx[M])N ⊳ 𝑀[𝑥:=𝑁]`, provided no variable that occurs free in N becomes bound after its substitution into M.

Example of α-convertibility and β-conversion
Let us consider the function: `λx[λy[x(y−5)]]`
If we wanted to apply the argument `2y` to this function, we couldn't, as that would violate the rule for β-conversion (y would become a bound variable, when it occurs free in N). Therefore, the following conversion would be illegal:
- `(λx[λy[x(y−5)]])2y ⊳ λy[2y(y−5)]`

Therefore, we have to apply α-convertibility and change the bound variable y. We could therefore do the following and replace y for z:
- `λx[λz[x(z−5)]]`

After applying α-convertibility, we can now apply β-conversion. This gives us the following valid conversion:
- `(λx[λz[x(z−5)]])2y ⊳ λz[2y(z−5)]`


## Combinators
A combinator is a λ-term with no free variables. There are many combinators that have proven useful in lambda calculus. Below are some of the most relevant ones.

| Name | Definition                                       | Comments                                                                                                                                                                                                                                                    |
| ---- | ------------------------------------------------ | ----------------------------------------------------------------------------------------------------------------------------------------------------------------------------------------------------------------------------------------------------------- |
| S    | `λx[λy[λz[xz(yz)]]]`                             | Substitute-and-apply operator. z ‘intervenes’ between x and y: instead of applying x to y, we apply xz to yz.                                                                                                                                               |
| K    | `λx[λy[x]]`                                      | Constant function. The value of KM is the constant function whose value for any argument is simply M.                                                                                                                                                       |
| I    | `λx[x]`                                          | The identity function (returns whatever value is provided)                                                                                                                                                                                                  |
| B    | `λx[λy[λz[x(yz)]]]`                              | Recall that ‘xyz𝑥𝑦𝑧’ is to be understood as (xy)z(𝑥𝑦)𝑧, so this combinator is not a trivial identity function.                                                                                                                                        |
| C    | `λx[λy[λz[xzy]]]`                                | Swaps an argument                                                                                                                                                                                                                                           |
| T    | `λx[λy[x]]`                                      | Truth value `true` (Identical to K)                                                                                                                                                                                                                         |
| F    | `λx[λy[y]]`                                      | Truth value `false`                                                                                                                                                                                                                                         |
| ω    | `λx[xx]`                                         | Self-application combinator                                                                                                                                                                                                                                 |
| Ω    | ωω (`λx[xx]λx[xx]`)                              | Self-application of the self-application combinator. Reduces to itself.<br>This is how recursion is defined. When passing `λx[xx]` to itself, it will apply that function twice. Since `x = λx[xx]`, we are essentially always repeating the term `λx[xx]`. |
| Y    | `λf[(λx[f(xx)])(λx[f(xx)]𝜆𝑓[(𝜆𝑥[𝑓(𝑥𝑥)])]` | The y combinator.  For every λ-term X, we have:<br>YX ⊳ `(λx[X(xx)])(λx[X(xx)])`<br>      ⊳ `X((λx[X(xx)])(λx[X(xx)])`<br><br>The terms YX and X(YX) reduce to a common term.                                                                               |
| Θ    | `(λx[λf[f(xxf)]])(λx[λf[f(xxf)]]`                | Turing’s fixed-point combinator. For every λ-term X, ΘX reduces to X(ΘX)                                                                                                                                                                                    |

### Notations

| Name      | Application                                                                                                                                                                                                                                                                   |
| --------- | ----------------------------------------------------------------------------------------------------------------------------------------------------------------------------------------------------------------------------------------------------------------------------- |
| `MN`      | The application of the function M𝑀 to the argument N𝑁.                                                                                                                                                                                                                      |
| `PQR`     | The application of the function PQ, which is itself the application of the function P to the argument Q, to R. The disambiguation rule allows us to read this term as follows: (PQ)R                                                                                          |
| `(λx[M])` | The λ term that binds the variable x in the body term M.<br>Some authors write `λx.M` or `λx⋅M`                                                                                                                                                                               |
| `M[x:=A]` | The λ-term that is obtained by substituting the λ-term A for all free occurrences of x inside M.<br>For example, suppose M is `λx[x+y]`, and A is z. When we perform the substitution `M[x:=A]`, we replace all occurrences of x with A, so `M[x:=A]` would become `λx[z+y]`. |
| M≡N       | The λ𝜆-terms M and N are identical: understood as sequences of symbols, M and N have the same length and corresponding symbols of the sequences are identical.                                                                                                               |

## How is it valuable in computer science?

From a definition from [StackOverflow](https://stackoverflow.com/questions/93526/what-is-a-y-combinator/94056#94056):
> A Y-combinator is a "functional" (a function that operates on other functions) that enables recursion, <u>when you can't refer to the function from within itself (?)</u>. In computer-science theory, it generalizes recursion, abstracting its implementation, and thereby <u>separating it from the actual work of the function in question (?)</u>. The benefit of not needing a compile-time name for the recursive function is sort of a bonus.

This is a typical scenario for lambda functions, as they cannot call themselves by name. Assigning a lambda function to a variable is a brittle solution, as the variable can be reassigned (in the case of Scala, using `val` would make this at least look a little better, but it is still not a permanent solution). To try to understand how the Y-Combinator works, let us use the factorial function as an example:

```c 
x == 0 ? 1: x * func(x - 1);
```

Consider that function `func` will do exactly the same thing as the lambda expression. Now we can go one step further and turn this into a function that receives another function to call.

```c
// A function that creates a factorial, but only if you pass in
// a function that does what the inner function is doing.
Func<Func<Double, Double>, Func<Double, Double>> fact =
  (recurs) =>
    (x) =>
      x == 0 ? 1 : x * recurs(x - 1);
```

This function takes a function as an argument and returns another function as its result. Notice, however, that it does not call itself. It calls the argument (x) passed into the outer function. To make this factorial, we need to pass the inner function (`recurs`) to itself, which is done when we call the second inner function with the argument `x`.

Putting this all together, we have the following:

```c
// One-argument Y-Combinator.
public static Func<T, TResult> Y<T, TResult>(Func<Func<T, TResult>, Func<T, TResult>> F)
{
  return
    t =>  // A function that...
      F(  // Calls the factorial creator, passing in...
        Y(F)  // The result of this same Y-combinator function call...
              // (Here is where the recursion is introduced.)
      )
      (t); // And passes the argument into the work function.
}
```

This last sentence on StackOverflow explains it well:
> Rather than the factorial calling itself, what happens is that the factorial calls the factorial generator (returned by the recursive call to Y-Combinator). And depending on the current value of t the function returned from the generator will either call the generator again, with t - 1, or just return 1, terminating the recursion.

And this is where the definition of Y-combinator comes from: A function whose output is another function.

---
# Sources
- https://plato.stanford.edu/entries/lambda-calculus/